Test/dafnydoc/doc1/M.dfy
@@ -2,8 +2,14 @@
 module {:options "--function-syntax:4"} TestModule {
 
   const c: int := 7 + 
-                    if true then 8 else 9*1 /** Number of items */
-  const cc: real
+                    if true then 8 else 9*1 /** Number of items. ALl of them. */
+
+  const {:myattribute} cc: real
+  // The distance.
+  const ccc: bool
+  /** Valid or not. */
+  const {:myattribute}{:otherattribute 5,6} cccc: A?
+    // The internal state.
 
   module MInner /** Hidden stuff */
   {}
@@ -13,12 +19,36 @@ module {:options "--function-syntax:4"} TestModule {
   /** Opaque type */
   type T
 
-  /** Enumeration */
+  /** Enumeration. Various options. */
   datatype D = A | B
 
 
-  /** Returns a constant */
+  /** Returns a constant. A special constant. */
   function f(): int { 42 }
+
+  function fif(): int 
+    // return a constant. A special constant.
+  { 42 }
+
+  twostate function tf(): int 
+    /** A two-state function */
+  { 42 }
+
+  predicate p() 
+    // Always true. Every time.
+    ensures p() == true
+  { true }
+
+  predicate pp() 
+    /** Always true. Every time. */
+    ensures p() == true
+  { true }
+
+  predicate ppp() 
+    // Always true. Every time.
+  { true }
+
+  least predicate lp() /** A copredicate */ { false }
 
   method bump(i: int) returns (j: int) 
     // increments input
@@ -26,8 +56,18 @@ module {:options "--function-syntax:4"} TestModule {
     return i + 1;
   }
 
-  class A {
-    var j: int
+  /** Sets to zero. Absolute zero. */
+  ghost method {:iszero} zero() returns (z: int) 
+    ensures z == 0
+  {
+    return 0;
+  }
+
+  class A 
+   // Holds all the state. Every bit.
+  {
+    var j: int // level
+    var k: D // options
     const c: int := 42
     method m(x: int)
       requires x > 0
@@ -37,7 +77,12 @@ module {:options "--function-syntax:4"} TestModule {
     predicate f<Q>() { true }
   }
 
-  lemma IsX()
+  lemma {:myattribute} IsX()
+    // always true
+    requires true
+    ensures true
+
+  twostate lemma TS()
     requires true
     ensures true
 }
